ohoh: done!

code/rocq/elpi.v
@@ -2,6 +2,7 @@ From mathcomp Require Import all_ssreflect.
 From det Require Import lang valid_state.
 From elpi.apps Require Import derive derive.std.
 From HB Require Import structures.
+From det Require Import zify_ssreflect.
 
 Section aux.
   Lemma ltn_leq_trans m n p :
@@ -135,13 +136,447 @@ End aux.
 
 Module Nur (U : Unif).
 
+  Class IsList {Th Tl : Type}  := {
+      nilC : Tl;
+      consC : Th -> Tl -> Tl;
+      appendC : Tl -> Tl -> Tl;
+      eqB : Tl -> Tl -> bool;
+      size   : Tl -> nat;
+      take   : nat -> Tl -> Tl;
+      drop   : nat -> Tl -> Tl;
+      behead : Tl -> Tl;
+      suffix : Tl -> Tl -> bool;
+      all: (Th -> bool) -> Tl -> bool;
+      map: (Th -> Th) -> Tl -> Tl;
+      mem: Th -> Tl -> bool;
+
+      cat_take_drop : forall (n0 : nat) s, appendC (take n0 s) (drop n0 s) = s;
+      cat_cons : forall x s1 s2, appendC (consC x s1) s2 = consC x (appendC s1 s2);
+      cats0  : forall (x: Tl), appendC x nilC = x;
+      cats20 : forall l1 l2, appendC l1 l2 = nilC -> l1 = nilC /\ l2 = nilC;
+      cat0s  : forall (x: Tl), appendC nilC x = x;
+      catA   : forall l1 l2 l3, appendC l1 (appendC l2 l3) = appendC (appendC l1 l2) l3;
+      suffix0s : forall l, suffix nilC l;
+      suffixs0 : forall l, suffix l nilC = (eqB l nilC);
+      take_size : forall s, take (size s) s = s;
+      drop_size : forall s, drop (size s) s = nilC;
+      size_nil: size nilC = 0;
+      drop0 l : drop 0 l = l;
+      take0 l : take 0 l = nilC;
+      drop_nil n : drop n nilC = nilC;
+      take_nil n : take n nilC = nilC;
+      eqb_refl l1: eqB l1 l1;
+      eqBP l1 l2: reflect (l1 = l2) (eqB l1 l2);
+      size_cat l1 l2: size (appendC l1 l2) = size l1 + size l2;
+      suffix_refl xs : suffix xs xs;
+      suffix_catr xs ys zs : suffix xs ys -> suffix xs (appendC zs ys);
+      take_size_cat n s1 s2: size s1 = n -> take n (appendC s1 s2) = s1;
+      drop_size_cat n s1 s2: size s1 = n -> drop n (appendC s1 s2) = s2;
+      behead_cons x xs: behead (consC x xs) = xs;
+      suffixP s1 s2: reflect (exists s2', s2 = appendC s2' s1) (suffix s1 s2);
+      size_suffix s1 s2: suffix s1 s2 -> size s1 <= size s2;
+      suffix_catl: forall s1 s2 s3 s3', size s3 = size s3' ->
+        suffix (appendC s1 s3) (appendC s2 s3') = (eqB s3 s3') && suffix s1 s2;
+      all_cat p l1 l2: all p (appendC l1 l2) = all p l1 && all p l2;
+      all_cons p x xs: all p (consC x xs) = p x && all p xs; 
+      size_cons x xs: size (consC x xs) = (size xs).+1;
+      map_cat F l1 l2 : map F (appendC l1 l2) = appendC (map F l1) (map F l2);
+      map_cons F l1 l2 : map F (consC l1 l2) = consC (F l1) (map F l2);
+      size_map F l1 : size (map F l1) = size l1;
+      map_id l1 : map id l1 = l1;
+      (* eq_in_map f g s: (forall x, mem x s -> f x = g x) <-> map f s = map g s *)
+    }.
+  Declare Scope SE.
+  Global Infix "++" := appendC : SE.
+  Open Scope SE.
+  Arguments appendC: simpl never.
+  Arguments nilC : simpl never.
+  Arguments consC : simpl never.
+  Arguments suffix : simpl never.
+  Arguments take : simpl never.
+  Arguments drop : simpl never.
+  Arguments size : simpl never.
+  Arguments eqB : simpl never.
+  Arguments behead : simpl never.
+  Arguments all : simpl never.
+  Arguments map : simpl never.
+
   Module VS := valid_state(U).
   Import VS RunP Run Language.
   
   Inductive G := 
     | call : program -> Tm -> G
-    | cut : list (list G) -> G
-    .
+    | cut : alts -> G
+  with alts :=
+    | no_alt
+    | more_alt : goals -> alts -> alts
+  with goals :=
+    | no_goals
+    | more_goals : G -> goals -> goals .
+
+  Fixpoint eqb_alts t1 t2 :=
+    match t1, t2 with
+    | no_alt, no_alt => true
+    | more_alt h1 t1, more_alt h2 t2 => eqb_goals h1 h2 && eqb_alts t1 t2
+    | _, _ => false
+    end
+  with eqb_goals t1 t2 :=
+    match t1, t2 with
+    | no_goals, no_goals => true
+    | more_goals h1 t1, more_goals h2 t2 => eqb_G h1 h2 && eqb_goals t1 t2
+    | _, _ => false
+    end
+  with eqb_G t1 t2 :=
+    match t1, t2 with
+    | call p1 t1, call p2 t2 => (p1 == p2) && (t1 == t2)
+    | cut ca1, cut ca2 => eqb_alts ca1 ca2
+    | _, _ => false
+    end.
+
+  Lemma eqb_reflA l : eqb_alts l l
+    with eqb_reflG l : eqb_goals l l
+    with eqb_G_refl l : eqb_G l l.
+  Proof.
+    {
+      case: l => /=.
+        move=>//.
+      move=> g gs; rewrite eqb_reflA eqb_reflG//.
+    }
+    case: l => /=.
+      move=>//.
+    move=> [p t|ca]/=gs; rewrite ?eqxx eqb_reflG//eqb_reflA//.
+    case: l => //=p t; rewrite !eqxx//.
+  Qed.
+
+  Lemma eqbPA l1 l2 : reflect (l1 = l2) (eqb_alts l1 l2)
+    with eqbPG l1 l2 : reflect (l1 = l2) (eqb_goals l1 l2)
+    with eqbP_G l1 l2 : reflect (l1 = l2) (eqb_G l1 l2).
+  Proof.
+    {
+      case: l1; case: l2 => /=.
+      - constructor => //.
+      - move=> g gx; constructor => //.
+      - move=> g gs; constructor => //.
+      - move=> x xs y ys.
+        case X: eqb_goals => /=.
+          case Y: eqb_alts => /=; constructor.
+            have:= eqbPA ys xs; rewrite Y.
+            inversion 1; subst.
+            have:= eqbPG y x; rewrite X.
+            inversion 1; subst => //.
+          have:= eqbPA ys xs; rewrite Y; inversion 1.
+          move=> [??]; subst; auto.
+        have:= eqbPG y x; rewrite X; inversion 1; constructor.
+        move=>[??]; subst; auto.
+    }
+    {
+      case: l1; case: l2 => /=.
+      - constructor => //.
+      - move=> g gx; constructor => //.
+      - move=> g gs; constructor => //.
+      - move=> x xs y ys.
+        case X: eqb_G => /=.
+          case Y: eqb_goals => /=; constructor.
+            have:= eqbPG ys xs; rewrite Y.
+            inversion 1; subst.
+            have:= eqbP_G y x; rewrite X.
+            inversion 1; subst => //.
+          have:= eqbPG ys xs; rewrite Y; inversion 1.
+          move=> [??]; subst; auto.
+        have:= eqbP_G y x; rewrite X; inversion 1; constructor.
+        move=>[??]; subst; auto.
+    }
+    case: l1 => [p t|ca].
+    - case X: eqb_G; constructor; case: l2 X => //=??.
+        move=>/andP[/eqP->/eqP->//].
+      move=> +[??]; subst; rewrite !eqxx//.
+    - case X: eqb_G; constructor; case: l2 X => //=ca' H.
+        have:= eqbPA ca ca'; rewrite H; inversion 1; subst => //.
+      have:= eqbPA ca ca'; rewrite H; inversion 1; subst; congruence.
+  Qed.
+     
+
+  Notation "x ::: xs" :=
+    (consC x xs)
+    (at level 3, no associativity)
+    : SE.
+
+  Notation "-[]" :=
+    (nilC)
+    (at level 3, no associativity,only printing)
+    : SE.
+
+  Notation "(( x ))" := (consC x nilC)
+    (at level 3, no associativity,only printing)
+    : SE.
+
+
+  Section alts.
+    Fixpoint append_alts l1 l2 := 
+      match l1 with
+      | no_alt => l2
+      | more_alt hd tl => more_alt hd (append_alts tl l2)
+      end.
+
+    Fixpoint all_alts p l :=
+      match l with
+      | no_alt => true
+      | more_alt hd tl => p hd && all_alts p tl
+      end.
+
+    Fixpoint size_alts l1 := 
+      match l1 with
+      | no_alt => 0
+      | more_alt _ l1 => (size_alts l1).+1
+      end.
+
+    Fixpoint take_alts n l1 :=
+      match n, l1 with
+      | 0, _ | _, no_alt => no_alt
+      | n.+1, more_alt x l => more_alt x (take_alts n l)
+      end.
+
+    Fixpoint drop_alts n l1 :=
+      match n, l1 with
+      | 0, l | _, (no_alt as l) => l
+      | n.+1, more_alt _ l => drop_alts n l
+      end.
+
+    Definition behead_alts l :=
+      match l with
+      | no_alt => no_alt
+      | more_alt _ l => l
+      end.
+
+    Fixpoint suffix_alts l1 l2 :=
+      if eqb_alts l1 l2 then true
+      else 
+      match l2 with
+      | no_alt => false
+      | more_alt x xs => suffix_alts l1 xs
+      end.
+
+    Lemma suffixPA s1 s2: reflect (exists s2', s2 = append_alts s2' s1) (suffix_alts s1 s2).
+    Proof.
+      elim: s2 s1 => //=.
+        move=>[|g gs]; constructor.
+          by exists no_alt.
+        by move=>[]-[]//.
+      move=> g gs IH s1.
+      case: ifP.
+        move=>/eqbPA->; constructor; exists no_alt => //.
+      move=> H.
+      have [H1|H1] := IH s1; constructor.
+        case: H1 => x->; exists (more_alt g x) => //.
+      move=> [x H2]; apply: H1.
+      case: x H2 => [|x xs]/=.
+        move=>?; subst.
+        rewrite eqb_reflA// in H.
+      move=>[_->]; exists xs => //.
+    Qed.
+
+    Lemma catAA x y z: append_alts x (append_alts y z) = append_alts (append_alts x y) z.
+    Proof. elim: x y z => //= x xs IH y z; rewrite IH//. Qed.
+
+    Lemma cats0A l: append_alts l no_alt = l.
+    Proof. elim: l => //= x xs ->//. Qed.  
+
+    Lemma size_cat_alts xs ys:
+      size_alts (append_alts xs ys) = (size_alts xs) + (size_alts ys).
+    Proof. elim: xs ys => //= _ xs IH ys; rewrite IH; lia. Qed.
+
+    Lemma suffix_catlA s1 s2 s3 s3':
+      size_alts s3 = size_alts s3' ->
+      suffix_alts (append_alts s1 s3) (append_alts s2 s3') = eqb_alts s3 s3' && suffix_alts s1 s2.
+    Proof.
+      elim: s3 s3' s1 s2 => //=.
+        move=>[]//= s1 s2; rewrite !cats0A//.
+      move=> g gs IH []//=y ys s1 s2 [H1].
+      have:= IH _ _ _ H1.
+      case: eqbPA => /=.
+        move=>?; subst.
+      Admitted.
+
+    Fixpoint mapA F l :=
+      match l with
+      | no_alt => no_alt
+      | more_alt x xs => more_alt (F x) (mapA F xs)
+      end.
+
+    Fixpoint memA e l := 
+      match l with
+      | no_alt => false
+      | more_alt x xs => eqb_goals e x || memA e xs
+      end.
+
+    #[refine] Global Instance IsList_alts : @IsList goals alts :=
+      {| 
+      nilC := no_alt; consC := more_alt;  
+      appendC := append_alts; size := size_alts; take := take_alts; drop := drop_alts;
+      behead := behead_alts; eqB := eqb_alts; suffix:= suffix_alts; all:= all_alts;
+      map := mapA; mem := memA
+      |}.
+    Proof.
+      all: try by move=> //.
+      move=> n; elim: n =>// n IH []//=g gs; rewrite IH//.
+      move=> l1; elim: l1 => //= x xs->//.
+      move=> l1; elim: l1 => //=x xs IH l2 l3; rewrite IH//.
+      move=> l1; elim: l1 => //=x xs IH l2 l3; rewrite IH//.
+      move=> l; elim: l => //.
+      move=> l; elim: l => //=x xs->//.
+      move=> l; elim: l => //=x xs->//.
+      move=> n; elim: n => //=.
+      move=> n; elim: n => //=.
+      move=> n; elim: n => //=.
+      apply: eqb_reflA.
+      apply: eqbPA.
+      apply: size_cat_alts.
+      move=> xs; elim: xs => //=x xs H; rewrite eqb_reflG eqb_reflA//.
+      move=> ++zs; elim: zs => //=x xs IH ys zs; case: ifP => // _; apply: IH.
+      move=> n; elim: n => [|n IH] []//=g xs ys []/IH->//.
+      move=> n; elim: n => [|n IH][]//= _ xs ys []/IH->//.
+      apply: suffixPA.
+      move=>s1 s2 /suffixPA [x ->]; rewrite size_cat_alts; lia.
+      apply: suffix_catlA.
+      move=> p l1; elim: l1 => //= g gs IH l2; rewrite IH -andbA//.
+      move=> F l1; elim: l1 => //=x xs IH l1; rewrite IH//.
+      move=> F l1; elim: l1 => //=_ xs->//.
+      move=>l; elim: l => //=g gs->//.
+      (* move=> f g s. *)
+    Defined.
+  End alts.
+
+  Section goals.
+    Fixpoint append_goals l1 l2 := 
+      match l1 with
+      | no_goals => l2
+      | more_goals hd tl => more_goals hd (append_goals tl l2)
+      end.
+
+    Fixpoint all_goals p l :=
+      match l with
+      | no_goals => true
+      | more_goals hd tl => p hd && all_goals p tl
+      end.
+
+    Fixpoint size_goals l1 := 
+      match l1 with
+      | no_goals => 0
+      | more_goals _ l1 => (size_goals l1).+1
+      end.
+
+    Fixpoint take_goals n l1 :=
+      match n, l1 with
+      | 0, _ | _, no_goals => no_goals
+      | n.+1, more_goals x l => more_goals x (take_goals n l)
+      end.
+
+    Fixpoint drop_goals n l1 :=
+      match n, l1 with
+      | 0, l | _, (no_goals as l) => l
+      | n.+1, more_goals _ l => drop_goals n l
+      end.
+
+    Definition behead_goals l :=
+      match l with
+      | no_goals => no_goals
+      | more_goals _ l => l
+      end.
+
+    Fixpoint suffix_goals l1 l2 :=
+      if eqb_goals l1 l2 then true
+      else 
+      match l2 with
+      | no_goals => false
+      | more_goals x xs => suffix_goals l1 xs
+      end.
+
+    Fixpoint mapG F l :=
+      match l with
+      | no_goals => no_goals
+      | more_goals x xs => more_goals (F x) (mapG F xs)
+      end.
+
+    Lemma suffixPG s1 s2: reflect (exists s2', s2 = append_goals s2' s1) (suffix_goals s1 s2).
+    Proof.
+      elim: s2 s1 => //=.
+        move=>[|g gs]; constructor.
+          by exists no_goals.
+        by move=>[]-[]//.
+      move=> g gs IH s1.
+      case: ifP.
+        move=>/eqbPG->; constructor; exists no_goals => //.
+      move=> H.
+      have [H1|H1] := IH s1; constructor.
+        case: H1 => x->; exists (more_goals g x) => //.
+      move=> [x H2]; apply: H1.
+      case: x H2 => [|x xs]/=.
+        move=>?; subst.
+        rewrite eqb_reflG// in H.
+      move=>[_->]; exists xs => //.
+    Qed.
+
+    Lemma catAG x y z: append_goals x (append_goals y z) = append_goals (append_goals x y) z.
+    Proof. elim: x y z => //= x xs IH y z; rewrite IH//. Qed.
+
+    Lemma cats0G l: append_goals l no_goals = l.
+    Proof. elim: l => //= x xs ->//. Qed.  
+
+    Lemma size_cat_goal xs ys:
+      size_goals (append_goals xs ys) = (size_goals xs) + (size_goals ys).
+    Proof. elim: xs ys => //= _ xs IH ys; rewrite IH; lia. Qed.
+
+    Lemma suffix_catlG s1 s2 s3 s3':
+      size_goals s3 = size_goals s3' ->
+      suffix_goals (append_goals s1 s3) (append_goals s2 s3') = eqb_goals s3 s3' && suffix_goals s1 s2.
+    Proof.
+      elim: s3 s3' s1 s2 => //=.
+        move=>[]//= s1 s2; rewrite !cats0G//.
+      move=> g gs IH []//=y ys s1 s2 [H1].
+      have:= IH _ _ _ H1.
+      case: eqbPG => /=.
+        move=>?; subst.
+      Admitted.
+
+    Fixpoint memG e l := 
+      match l with
+      | no_goals => false
+      | more_goals x xs => eqb_G e x || memG e xs
+      end.    
+
+    #[refine] Global Instance IsList_goals : @IsList G goals :=
+      {| nilC := no_goals; consC := more_goals; map:= mapG;
+         appendC := append_goals; size := size_goals; take:= take_goals; drop := drop_goals;
+         behead := behead_goals; suffix := suffix_goals; eqB := eqb_goals; all:= all_goals;
+         mem := memG |}.
+    Proof.
+      all: try by move=>//.
+      move=> n; elim: n =>// n IH []//=g gs; rewrite IH//.
+      move=> l1; elim: l1 => //= x xs->//.
+      move=> l1; elim: l1 => //=x xs IH l2 l3; rewrite IH//.
+      move=> l1; elim: l1 => //=x xs IH l2 l3; rewrite IH//.
+      move=> l; elim: l => //.
+      move=> l; elim: l => //=x xs->//.
+      move=> l; elim: l => //=x xs->//.
+      move=> n; elim: n => //.
+      move=> n; elim: n => //.
+      move=> n; elim: n => //.
+      apply: eqb_reflG.
+      apply: eqbPG.
+      move=> l1; elim: l1 => //= _ x IH l2; rewrite IH; lia.
+      move=> xs; elim: xs => //=x xs H; rewrite eqb_reflG eqb_G_refl//.
+      move=> ++zs; elim: zs => //=x xs IH ys zs; case: ifP => // _; apply: IH.
+      move=> n; elim: n => [|n IH] []//=g xs ys []/IH->//.
+      move=> n; elim: n => [|n IH][]//= _ xs ys []/IH->//.
+      apply: suffixPG.
+      move=>s1 s2 /suffixPG [x ->]; rewrite size_cat_goal; lia.
+      apply: suffix_catlG.
+      move=> p l1; elim: l1 => //= g gs IH l2; rewrite IH -andbA//.
+      move=> F l1; elim: l1 => //=x xs IH l1; rewrite IH//.
+      move=> F l1; elim: l1 => //=_ xs->//.
+      move=> l; elim: l => //=x xs->//.
+    Defined.
+  End goals.
 
   Definition if_cut F g :=
     match g with
@@ -155,21 +590,6 @@ Module Nur (U : Unif).
     | _ => g
     end.
 
-  derive G.
-  HB.instance Definition _ := hasDecEq.Build G G_eqb_OK.
-
-  Definition alt := (list G).
-
-  Definition a2g p A :=
-    match A with
-    | Cut => cut [::]
-    | Call t => call p t
-    end.
-
-  Definition a2gs p (b : Sigma * R) :=
-    map (a2g p) b.2.(premises).
-
-  Section add_ca.
 
     Definition add_ca alts a :=
       match a with
@@ -177,34 +597,66 @@ Module Nur (U : Unif).
       | call pr t => call pr t
       end.
 
-    Lemma add_ca_empty {T: Type} (F: T -> G) {lA}:
-      map (fun i => add_ca [::] (F i)) lA = map F lA.
-    Proof.
-      rewrite /add_ca; elim: lA => //= x xs ->; f_equal.
-      case: F => //l; rewrite cats0//.
-    Qed.
+    Fixpoint add_ca_deep (bt:alts) (ats: alts) : alts :=
+      match ats with
+      | no_alt => nilC
+      | more_alt hd tl => (add_ca_deep_goals bt hd) ::: (add_ca_deep bt tl)
+      end
+    with add_ca_deep_goals bt gl :=
+      match gl with
+      | no_goals => nilC 
+      | more_goals hd tl => (add_ca_deep_g bt hd) ::: (add_ca_deep_goals bt tl)
+      end
+    with add_ca_deep_g bt g := (*if ca == [::] then behaves like add_ca *)
+      match g with
+      | call pr t => call pr t 
+      | cut ca => cut ((add_ca_deep bt ca) ++ bt)
+      end.
 
-    Lemma map_add0_cas_empty {T:Type} (F: T -> G) {lA}:
-      map (map (fun i => add_ca [::] (F i))) lA  = map (map F) lA.
-    Proof.
-      rewrite /add_ca; elim: lA => //= x xs ->.
-      f_equal; apply add_ca_empty.
-    Qed.
-  End add_ca.
+  Definition save_goals (a: alts) (gs b:goals) := map (add_ca a) b ++ gs.
+
+  Definition save_alts (a : alts) (gs: goals) (bs : alts) := map (save_goals a gs) bs.
 
 
-  Definition save_alt a gs b := map (add_ca a) b ++ gs.
-  Definition more_alt a gs bs := map (save_alt a gs) bs.
+  (* Definition points_to l1 A := match A with cut l2 => l1 == l2 | _ => true end. *)
+  (* Definition empty_ca := points_to [::]. *)
 
-  Inductive nur : Sigma -> list G ->  list alt -> Sigma -> list alt -> Prop :=
-  | StopE s a : nur s [::] a s a
-  | CutE s s1 a ca r gl : nur s gl ca s1 r -> nur s [:: cut ca & gl] a s1 r
+  Definition empty_ca_G g :=
+    match g with call _ _ | cut no_alt => true | _ => false end.
+  Definition empty_caG goals := all empty_ca_G goals.
+  Definition empty_ca alts := all empty_caG alts.
+
+  Definition a2g p A :=
+    match A with
+    | Cut => cut nilC
+    | Call t => call p t
+    end.
+
+  Fixpoint a2gs p (b: seq A) := 
+    match b with
+    | nil => nilC
+    | x::xs => (a2g p x) ::: (a2gs p xs)
+    end.
+
+  Fixpoint aa2gs p (b: (seq (Sigma * R))) := 
+    match b with
+    | nil => nilC
+    | x::xs => (a2gs p x.2.(premises)) ::: (aa2gs p xs)
+    end.
+
+  Definition a2gs1 p (b : Sigma * R) :=
+    a2gs p b.2.(premises).
+
+
+  Inductive nur : Sigma -> goals ->  alts -> Sigma -> alts -> Prop :=
+  | StopE s a : nur s nilC a s a
+  | CutE s s1 a ca r gl : nur s gl ca s1 r -> nur s ((cut ca) ::: gl) a s1 r
   | CallE p s s1 a b bs gl r t : 
     F p t s = [:: b & bs ] -> 
-      nur s (save_alt a gl (a2gs p b)) (more_alt a gl (map (a2gs p) bs) ++ a) s1 r -> 
-        nur s [::call p t & gl] a s1 r
+      nur s (save_goals a gl (a2gs1 p b)) (save_alts a gl ((aa2gs p) bs) ++ a) s1 r -> 
+        nur s ((call p t) ::: gl) a s1 r
   | FailE p s s1 t gl a al r : 
-    F p t s = [::] -> nur s a al s1 r -> nur s [::call p t & gl] (a :: al) s1 r.
+    F p t s = [::] -> nur s a al s1 r -> nur s ((call p t) ::: gl) (a ::: al) s1 r.
 
   Lemma nur_consistent {s G x xs1 xs2 s1 s2} :
     nur s G x s1 xs1 -> nur s G x s2 xs2 -> xs1 = xs2 /\ s1 = s2.
@@ -226,7 +678,7 @@ Module Nur (U : Unif).
   Definition get_ca g :=
     match g with
     | cut a => a 
-    | _ => [::]
+    | _ => nilC
     end.
 
   Definition is_cutb' A := match A with cut _ => true | _ => false end.
@@ -235,60 +687,36 @@ Module Nur (U : Unif).
   Lemma cuts_cat {x y} : cuts' (x ++ y) = cuts' x && cuts' y.
   Proof. rewrite/cuts' all_cat//. Qed.
 
-  Fixpoint add_ca_deep n tl (alts: seq (seq G)) := (*always:= adds always alts to cut *)
-    match n with
-    | 0 => alts
-    | n.+1 => map (map (fun x => (add_ca tl (apply_cut (add_ca_deep n tl) x)))) alts
-    end.
-
-  (* Definition add_ca1 tl a := add_ca_deep (size a) tl a. *)
-
-  Lemma add_ca_empty1 l: add_ca [::] l = l.
+  Lemma add_ca_empty1 l: add_ca nilC l = l.
   Proof. case: l => //= l1; rewrite cats0//. Qed.
-
-  Lemma map_add1_cas_empty {T: Type} (lA: (list T)) F:
-    (map (fun x => add_ca [::] (F x))) lA  = (map F) lA.
-  Proof.
-    rewrite /add_ca; elim: lA => //= x xs ->.
-    case: (F x)=>//=l; rewrite cats0//.
-  Qed.
-
-
-  Lemma map_map_add1_cas_empty {T: Type} (lA: list (list T)) F:
-    map (map (fun x => add_ca [::] (F x))) lA  = map (map F) lA.
-  Proof.
-    rewrite /add_ca; elim: lA => //= x xs ->.
-    f_equal; apply: map_add1_cas_empty.
-  Qed.
 
   Lemma cut_add_ca {l x}: is_cutb' (add_ca l x) = is_cutb' x.
   Proof. case: x => //=*. Qed.
 
-  Lemma cuts_add_ca {x l} : cuts' [seq add_ca l j | j <- x] = cuts' x.
-  Proof. elim: x l => // x xs H/= l; rewrite H cut_add_ca//. Qed.
+  Definition make_lB0 (xs:alts) (lB0: goals) := map (fun x => x ++ lB0) xs.
+  
+  Definition make_lB01 (xs:alts) (lB0: goals) := map (fun x => lB0 ++ x) xs.
 
-  Definition make_lB0 (xs:seq alt) (lB0: alt) := map (fun x => x ++ lB0) xs.
-
-  Definition add_deep_help add_deep (bt:seq alt) (n:nat) hd :=
-    apply_cut (fun x =>
-      let s := size x - size bt in
-      make_lB0 (add_deep bt n hd (take s x)) hd ++ drop s x).
-
-  Fixpoint add_deep bt n (l: alt) (A: seq alt) :=
-    match n with
-    | 0 => A
-    | n.+1 =>
-      map (map (add_deep_help add_deep bt n l)) A
-    end. 
-
-  Definition add_deep_ bt n (l: alt) (A: alt) :=
-    match n with
-    | 0 => A
-    | n.+1 => (map (add_deep_help add_deep bt n l)) A
+  Fixpoint add_deep (bt: alts) (l: goals) (A : alts) : alts :=
+    match A with
+    | no_alt => nilC
+    | more_alt hd tl => (add_deepG bt l hd) ::: (add_deep bt l tl)
+    end
+    with add_deepG (bt: alts) (l: goals) (A : goals) :=
+    match A with
+    | no_goals => nilC
+    | more_goals hd tl => (add_deep_G bt l hd) ::: (add_deepG bt l tl)
+    end
+    with add_deep_G bt l A :=
+    match A with
+    | cut ca => 
+      let s := size ca - size bt in
+      let xx := (add_deep bt l (ca)) in
+      cut (make_lB0 (take s xx) l ++ drop s ca)
+    | call pr t => call pr t 
     end.
 
-  Definition kill (A: alt) := map (apply_cut (fun x => [::])) A.
-
+  Definition kill (A: goals) := map (apply_cut (fun x => nilC)) A.
 
     (* bt is the backtracking list for the cut-alternatives
       this list is important since in this tree:
@@ -302,44 +730,47 @@ Module Nur (U : Unif).
       the "great^n uncles" on the right of a cut ARE alternatives
     *)
 
-  Fixpoint state_to_list (A: state) (bt : list alt) : list alt :=
+  Fixpoint state_to_list (A: state) (bt : alts) : alts :=
     match A with
-    | OK => [::[::]]
-    | Top => [::[::]]
-    | Bot => [::]
-    | Dead => [::]
-    | Goal _ Cut => [::[::cut [::]]]
-    | Goal pr (Call t) => [::[::call pr t]]
+    | OK => (nilC) ::: nilC
+    | Top => (nilC) ::: nilC
+    | Bot => nilC
+    | Dead => nilC
+    | Goal _ Cut => ((cut nilC) ::: nilC) ::: nilC
+    | Goal pr (Call t) => ((call pr t) ::: nilC) ::: nilC
     | Or A _ B => 
-      let lB := state_to_list B [::] in
+      let lB := state_to_list B nilC in (*lB = (call p t :: gs) :: a*)
       let lA := state_to_list A lB in
-      add_ca_deep (size (lA ++ lB)) bt (lA ++ lB)
+      (* add_ca_deep (size (lB)) bt (lB) *)
+      add_ca_deep bt (lA ++ lB)
     | And A B0 B =>
       let lB0 := state_to_list B0 bt in
       let lA   := state_to_list A bt in
-      if lA is x :: xs then 
+      if lA is more_alt x xs then 
         (* lA is split into the current goal x and the future alternatives xs *)
         (* in a valid state lB0 has length 0 or 1 (it is a (potentially killed) base and) *)
         match lB0 with
-        | [::] => 
+        | no_alt => 
           (* the reset point is empty: it kill all the alternatives in the cut-to *)
           let lB   := state_to_list B bt in
-          [seq (kill x) ++ y | y <- lB]
-        | [::hd] =>
+          make_lB01 lB (kill x)
+
+          (* [seq (kill x) ++ y | y <- lB] *)
+        | more_alt hd no_alt =>
         (* 
           invariant every cut-to has bt has tail or is empty
         *)
           (* the reset point exists, it has to be added to all cut-to alternatives *)
-          let x := add_deep_ bt (size xs).+1 hd x in
-          let xs := add_deep bt (size xs) hd xs in 
+          let x := add_deepG bt hd x in
+          let xs := add_deep bt hd xs in 
           (* each alt in xs must have hd has rightmost conjunct  *)
           let xs := make_lB0 xs hd in
           (* xs are alternatives that should be added in the deep cuts in B *)
           let lB   := state_to_list B (xs ++ bt) in
           (* lB are alternatives, each of them have x has head *)
-          [seq x ++ y | y <- lB] ++ xs
-        | _ => [::] (*unreachable in a valid_state*)
+          make_lB01 lB x ++ xs
+        | _ => nilC (*unreachable in a valid_state*)
         end
-      else [::]
+      else nilC
     end.
 End Nur.
